use cbor_copy_t

src/cbor/pulse/raw/CBOR.Pulse.API.Det.C.Copy.fst
@@ -17,7 +17,7 @@ let freeable = Copy.freeable
 let cbor_get_from_freeable x = Copy.Mkcbor_freeable?.cbor x
 
   fn cbor_copy (_: unit)
-: cbor_det_copy_t
+: cbor_copy_t cbor_det_match freeable cbor_get_from_freeable
 =
   (c: _)
   (#p: _)
